frodo/code/Hacl.Impl.Frodo.Sample.fst
@@ -4,8 +4,6 @@ open FStar.HyperStack
 open FStar.HyperStack.ST
 open FStar.Mul
 
-open LowStar.Buffer
-
 open Lib.IntTypes
 open Lib.Buffer
 open Lib.ByteBuffer
@@ -14,14 +12,18 @@ open Hacl.Impl.Matrix
 open Hacl.Impl.Frodo.Params
 
 module ST = FStar.HyperStack.ST
-module HS = FStar.HyperStack
 module Lemmas = Spec.Frodo.Lemmas
+module Seq = Lib.Sequence
 module S = Spec.Frodo.Sample
-module B = LowStar.Buffer
 
-#reset-options "--z3rlimit 50 --max_fuel 0 --max_ifuel 0 --using_facts_from '*'"
+#reset-options "--z3rlimit 50 --max_fuel 0 --max_ifuel 0"
 
-let cdf_table = icreateL_global cdf_list
+let cdf_seq: Seq.lseq uint16 (v cdf_table_len) = 
+  assert_norm (List.Tot.length cdf_list == v cdf_table_len);
+  Seq.of_list cdf_list
+
+let cdf_table: b:ilbuffer uint16 cdf_table_len{recallable b /\ witnessed b cdf_seq} = 
+  createL_global cdf_list
 
 inline_for_extraction noextract
 val frodo_sample_f:
@@ -29,12 +31,11 @@ val frodo_sample_f:
   -> i:size_t{v i < v cdf_table_len}
   -> Stack uint16
      (requires fun h -> True)
-     (ensures  fun h0 r h1 ->
-       modifies loc_none h0 h1 /\ uint_v r == S.frodo_sample_f t (v i))
+     (ensures  fun h0 r h1 -> modifies0 h0 h1 /\ uint_v r == S.frodo_sample_f t (v i))
 let frodo_sample_f t i =
   assert_norm (List.Tot.length cdf_list <= max_size_t);
-  recall_contents cdf_table (Seq.seq_of_list cdf_list);
-  let ti = iindex cdf_table (Lib.RawIntTypes.size_to_UInt32 i) in
+  recall_contents cdf_table cdf_seq;
+  let ti = index cdf_table (Lib.RawIntTypes.size_to_UInt32 i) in
   S.lemma_frodo_sample0 (v i);
   S.lemma_frodo_sample1 t ti;
   to_u16 (to_u32 (ti -. t)) >>. 15ul
@@ -45,15 +46,14 @@ val frodo_sample_res:
   -> sample:uint16{uint_v sample < v cdf_table_len}
   -> res:uint16{res == S.frodo_sample_res sign (uint_v sample)}
 let frodo_sample_res sign sample =
-  Spec.Frodo.Lemmas.lemma_frodo_sample2 sign sample;
+  Lemmas.lemma_frodo_sample2 sign sample;
   ((lognot sign +. u16 1) ^. sample) +. sign
 
 #set-options "--max_fuel 1"
 
 val frodo_sample: r:uint16 -> Stack uint16
   (requires fun h -> True)
-  (ensures  fun h0 res h1 ->
-    modifies loc_none h0 h1 /\ res == S.frodo_sample r)
+  (ensures  fun h0 res h1 -> modifies0 h0 h1 /\ res == S.frodo_sample r)
 [@"c_inline"]
 let frodo_sample r =
   push_frame();
@@ -62,19 +62,18 @@ let frodo_sample r =
   mod_mask_lemma r 1ul;
   uintv_extensionality (mod_mask 1ul) (u16 1);
   assert (uint_v sign == 0 \/ uint_v sign == 1);
-  let sample = create #uint16 #1 1ul (u16 0) in
+  let sample :lbuffer uint16 1ul = create (size 1) (u16 0) in
   let h = ST.get () in
-  assert (Lib.Sequence.index #_ #1 (as_seq h sample) 0 == u16 0);
-  assert (B.get h sample 0 == u16 0);
+  assert (Seq.index #_ #1 (as_seq h sample) 0 == u16 0);
+  assert (bget h sample 0 == u16 0);
   let bound = cdf_table_len -! 1ul in
   let h0 = ST.get () in
   Lib.Loops.for 0ul bound
-  (fun h i -> modifies (loc_buffer sample) h0 h /\
-    uint_v (B.get h sample 0) == S.frodo_sample_fc prnd i)
+  (fun h i -> modifies1 sample h0 h /\ v (bget h sample 0) == S.frodo_sample_fc prnd i)
   (fun i ->
-    let sample0 = sample.(0ul) in
-    let samplei = frodo_sample_f prnd i in
-    sample.(0ul) <- samplei +. sample0
+   let sample0 = sample.(0ul) in
+   let samplei = frodo_sample_f prnd i in
+   sample.(0ul) <- samplei +. sample0
   );
   let sample0 = sample.(0ul) in
   assert (uint_v sample0 == S.frodo_sample_fc prnd (v bound));
@@ -88,13 +87,13 @@ inline_for_extraction noextract
 val frodo_sample_matrix1:
     n1:size_t
   -> n2:size_t{0 < 2 * v n1 * v n2 /\ 2 * v n1 * v n2 <= max_size_t}
-  -> r:lbuffer uint8 (2 * v n1 * v n2)
+  -> r:lbuffer uint8 (size 2 *! n1 *! n2)
   -> i:size_t{v i < v n1}
   -> res:matrix_t n1 n2
   -> Stack unit
     (requires fun h -> live h r /\ live h res /\ disjoint r res)
     (ensures  fun h0 _ h1 ->
-      modifies (loc_buffer res) h0 h1 /\
+      modifies1 res h0 h1 /\
       as_matrix h1 res ==
       S.frodo_sample_matrix1 (v n1) (v n2) (as_seq h0 r) (v i) (as_matrix h0 res))
 let frodo_sample_matrix1 n1 n2 r i res =
@@ -119,7 +118,7 @@ val frodo_sample_matrix:
   -> Stack unit
     (requires fun h -> live h seed /\ live h res /\ disjoint seed res)
     (ensures  fun h0 r h1 ->
-      live h1 res /\ modifies (loc_buffer res) h0 h1 /\
+      live h1 res /\ modifies1 res h0 h1 /\
       as_matrix h1 res ==
       S.frodo_sample_matrix (v n1) (v n2) (v seed_len) (as_seq h0 seed) ctr)
 [@"c_inline"]
@@ -127,10 +126,9 @@ let frodo_sample_matrix n1 n2 seed_len seed ctr res =
   push_frame();
   let r = create (2ul *! n1 *! n2) (u8 0) in
   cshake_frodo seed_len seed ctr (2ul *! n1 *! n2) r;
-
   memset res (u16 0) (n1 *! n2);
   let h0 = ST.get () in
-  Lib.Sequence.eq_intro (Lib.Sequence.sub (as_seq h0 res) 0 (v n1 * v n2)) (as_seq h0 res);
+  Seq.eq_intro (Seq.sub (as_seq h0 res) 0 (v n1 * v n2)) (as_seq h0 res);
   [@ inline_let]
   let spec h0 = S.frodo_sample_matrix1 (v n1) (v n2) (as_seq h0 r) in
   let h0 = ST.get () in
